books/kestrel/helpers/package.lsp
@@ -1,0 +1,17 @@
+; The HELP package
+;
+; Copyright (C) 2022 Kestrel Institute
+;
+; License: A 3-clause BSD license. See the file books/3BSD-mod.txt.
+;
+; Author: Eric Smith (eric.smith@kestrel.edu)
+
+;;;;;;;;;;;;;;;;;;;;;;;;;;;;;;;;;;;;;;;;;;;;;;;;;;;;;;;;;;;;;;;;;;;;;;;;;;;;;;;;
+
+(in-package "ACL2")
+
+(defpkg "HELP" (append '(b*
+                         when ; the b* binder
+                         *t*
+                         *nil*)
+                       *acl2-exports*))
